define Ord Array

src/Init/Data/Ord.lean
@@ -666,6 +666,66 @@ theorem List.compare_nil_right_eq_eq {α} [Ord α] {xs : List α} :
 
 end List
 
+namespace Array
+
+variable {α}
+
+@[specialize]
+protected def compareLex {α} (cmp : α → α → Ordering) (a₁ a₂ : Array α) : Ordering :=
+  go 0
+where go i :=
+  if h₁ : a₁.size <= i then
+    if a₂.size <= i then .eq else .lt
+  else
+    if h₂ : a₂.size <= i then
+      .gt
+    else match cmp a₁[i] a₂[i] with
+      | .lt => .lt
+      | .eq => go (i + 1)
+      | .gt => .gt
+termination_by a₁.size - i
+
+instance {α} [Ord α] : Ord (Array α) where
+  compare := Array.compareLex compare
+
+protected theorem compare_eq_compareLex {α} [Ord α] :
+    compare (α := Array α) = Array.compareLex compare := rfl
+
+private theorem compareLexGo_succ {α} {cmp} {x₁ x₂} {a₁ a₂ : List α} {i} :
+    compareLex.go cmp (x₁ :: a₁).toArray (x₂ :: a₂).toArray (i + 1) =
+      compareLex.go cmp a₁.toArray a₂.toArray i := by
+  induction i using Array.compareLex.go.induct cmp a₁.toArray a₂.toArray
+  all_goals try
+    conv => congr <;> rw [compareLex.go]
+    simp
+    repeat' split <;> (try simp_all; done)
+
+private theorem compareLex_toArray_eq_listCompareLex {α} {cmp} {l₁ l₂ : List α} :
+    Array.compareLex cmp l₁.toArray l₂.toArray = List.compareLex cmp l₁ l₂ := by
+  simp only [Array.compareLex]
+  induction l₁ generalizing l₂ with
+  | nil =>
+    cases l₂
+    · simp [Array.compareLex.go, List.compareLex_nil_nil]
+    · simp [Array.compareLex.go, List.compareLex_nil_cons]
+  | cons x xs ih =>
+    cases l₂
+    · simp [Array.compareLex.go, List.compareLex_cons_nil]
+    · rw [Array.compareLex.go, List.compareLex_cons_cons]
+      simp only [List.size_toArray, List.length_cons, Nat.le_zero_eq, Nat.add_one_ne_zero,
+        ↓reduceDIte, List.getElem_toArray, List.getElem_cons_zero, Nat.zero_add]
+      split <;> simp_all [compareLexGo_succ]
+
+protected theorem compareLex_eq_compareLex_toList {α} {cmp} {a₁ a₂ : Array α} :
+    Array.compareLex cmp a₁ a₂ = List.compareLex cmp a₁.toList a₂.toList := by
+  rw [← compareLex_toArray_eq_listCompareLex]
+
+protected theorem compare_eq_compare_toList {α} [Ord α] {a₁ a₂ : Array α} :
+    compare a₁ a₂ = compare a₁.toList a₂.toList :=
+  Array.compareLex_eq_compareLex_toList
+
+end Array
+
 /-- The lexicographic order on pairs. -/
 def lexOrd [Ord α] [Ord β] : Ord (α × β) where
   compare := compareLex (compareOn (·.1)) (compareOn (·.2))
